\documentclass{article}

% Packages for formatting
\usepackage[margin=1in]{geometry}
\usepackage{fancyhdr}
\usepackage{enumitem}
\usepackage{graphicx}
\usepackage{kotex}
\usepackage{amsmath}
\usepackage{amsthm}
\usepackage{algorithm2e,setspace}
\usepackage{algpseudocode}
\usepackage{xcolor}
\usepackage{amssymb}

% Fonts
\usepackage[T1]{fontenc}
\usepackage[utf8]{inputenc}
\usepackage{newpxtext,newpxmath}
\usepackage{sectsty}

% Define colors
\definecolor{blue1}{HTML}{0077c2}
\definecolor{blue2}{HTML}{00a5e6}
\definecolor{blue3}{HTML}{b3e0ff}
\definecolor{blue4}{HTML}{00293c}
\definecolor{blue5}{HTML}{e6f7ff}

\definecolor{thmcolor}{RGB}{231, 76, 60}
\definecolor{defcolor}{RGB}{52, 152, 219}
\definecolor{lemcolor}{RGB}{155, 89, 182}
\definecolor{corcolor}{RGB}{46, 204, 113}
\definecolor{procolor}{RGB}{241, 196, 15}

\usepackage{color,soul}
\usepackage{soul}
\newcommand{\mathcolorbox}[2]{\colorbox{#1}{$\displaystyle #2$}}
\usepackage{cancel}
\newcommand\crossout[3][black]{\renewcommand\CancelColor{\color{#1}}\cancelto{#2}{#3}}
\newcommand\ncrossout[2][black]{\renewcommand\CancelColor{\color{#1}}\cancel{#2}}

\usepackage{hyperref}

% Chapter formatting
\definecolor{titleblue}{RGB}{0,53,128}
\usepackage{titlesec}
\titleformat{\section}
{\normalfont\sffamily\Large\bfseries\color{titleblue!100!gray}}{\thesection}{1em}{}
\titleformat{\subsection}
{\normalfont\sffamily\large\bfseries\color{titleblue!50!gray}}{\thesubsection}{1em}{}

%Tcolorbox
\usepackage[most]{tcolorbox}

%Tikzpicture
\usepackage{tikz-cd}
\usetikzlibrary{positioning}



% Header and footer formatting
\pagestyle{fancy}
\fancyhead{}
\fancyhf{}
\rhead{Student ID: 20192250\quad Name: 지용현}%\rule{3cm}{0.4pt}}
\lhead{\textcolor{blue2}{\textbf{PKC Assignment \#2}}}
% Define footer
\newcommand{\footer}[1]{
\begin{flushright}
	\vspace{2em}
	\includegraphics[width=2cm]{school_logo.jpg} \\
	\vspace{1em}
	\textcolor{blue2}{\small\textbf{#1}}
\end{flushright}
}
%\rfoot{\large Department of Information Security, Cryptogrphy and Mathematics, Kookmin Uni.\includegraphics[height=1.5cm]{school_logo.jpg}}
\fancyfoot{}
\fancyfoot[C]{-\thepage-}

\newcommand{\ie}{\textnormal{i.e.}}
\newcommand{\rsa}{\mathsf{RSA}}
\newcommand{\rsacrt}{\mathsf{RSA}\textendash\mathsf{CRT}}
\newcommand{\inv}[1]{#1^{-1}}

\usepackage{amsthm}
\newtheorem{axiom}{Axiom}[section]
\newtheorem{theorem}{Theorem}
\newtheorem*{theorem*}{Theorem}
\newtheorem{proposition}[theorem]{Proposition}
\newtheorem{corollary}{Corollary}[theorem]
\newtheorem*{corollary*}{Corollary}
\newtheorem{lemma}[theorem]{Lemma}
\newtheorem*{lemma*}{Lemma}

\theoremstyle{definition}
\newtheorem{definition}{Definition}
\newtheorem{remark}{Remark}
\newtheorem{exercise}{Exercise}[section]

%New Command
\newcommand{\set}[1]{\left\{#1\right\}}
\newcommand{\N}{\mathbb{N}}
\newcommand{\Z}{\mathbb{Z}}
\newcommand{\Q}{\mathbb{Q}}
\newcommand{\R}{\mathbb{R}}
\newcommand{\C}{\mathbb{C}}
\newcommand{\F}{\mathbb{F}}
\newcommand{\nbhd}{\mathcal{N}}

\newcommand{\of}[1]{\left( #1 \right)}

\begin{document}
\pagenumbering{arabic}
\begin{center}
	\huge\textbf{Public Key Cryptography}\\
	\vspace{0.5em}
\end{center}

\section{Chinese Remainder Theorem ($\mathsf{CRT}$)}

\begin{tcolorbox}[colback=white,colframe=lemcolor,arc=5pt,title={\hypertarget{lem}{}\color{white}\bf Bézout's Identity}]
	\begin{lemma*}
		$a,b\in\Z\implies\exists x,y\in\Z:\gcd\of{a,b}=ax+by$.
	\end{lemma*}
\end{tcolorbox}

\begin{tcolorbox}[colback=white,colframe=thmcolor,arc=5pt,title={\color{white}\bf Chinese Remainder Theorem ($\mathsf{CRT}$)}]
	\begin{theorem*}
		Given a system of $k$ linear congruences:
		\begin{align*}
			x&\equiv a_1 \pmod{m_1}\\
			x&\equiv a_2 \pmod{m_2}\\
			&\vdots \\
			x&\equiv a_k \pmod{m_k}
		\end{align*} where \textcolor{magenta}{$m_1,m_2,\dots, m_k$ are pairwise coprime}. Let $M=\prod_{i=1}^km_i$. Then, the \textcolor{red}{unique} \textcolor{blue}{solution} of the system of congruences is given by \begin{align*}
			X&\equiv\sum_{i=1}^ka_iM_ib_i\pmod{M}\\
			&\equiv a_1M_1b_1+a_2M_2b_2+\cdots+a_kM_kb_k\pmod{M}.
		\end{align*} where $M_i=M/m_i$ and $ b_i\equiv\inv{M_i}\pmod{m_i}$.
	\end{theorem*}
\end{tcolorbox}
\begin{proof}
	(\textcolor{blue}{Existence}) Define \begin{align*}
		M&:=\prod_{i=1}^km_i=m_1m_2\cdots m_k\quad\text{and}\\
		M_i&:=\frac{M}{m_i}=m_1m_2\cdots m_{i-1}m_{i+1}\cdots m_k.
	\end{align*} By Bézout's identity, we know that \[
	\exists b_i,c_i\in\Z: M_ib_i+m_ic_i=\gcd\of{M_i,m_i}=1.
	\] because $M_i$ has not $m_i$ as factor. Note that \begin{itemize}
		\item[(1)] $M_ib_i+m_ic_i=1\Leftrightarrow M_ib_i=(-c_i)m_i+1\Leftrightarrow M_1b_i\equiv 1\pmod{m_i}$.
		\item[(2)] Let $i,j\in\set{1,2,\cdots, k}$ with $i\neq j$. Then\begin{align*}
			\textcolor{magenta}{\gcd\of{m_i,m_j}=1}&\implies m_j\in\set{m_1,m_2,\cdots,m_{i-1},m_{i+1},\cdots,m_k}\\
			&\implies m_j\mid M_i\quad\because M_i=m_1m_2\cdots m_{i-1}m_{i+1}\cdots m_k\\
			&\implies m_j\mid M_i-0\\
			&\implies M_i\equiv 0\pmod{m_j}.
		\end{align*}
	\end{itemize} 
	Thus, we have \[
	\begin{cases}
		M_ib_i\equiv 1\pmod{m_i}\quad\cdots\cdots(1)\\
		M_ib_i\equiv 0\pmod{m_j}\ \text{for $j\neq i$}\quad\cdots\cdots(2).
	\end{cases}
	\] 
	Then we claim that $X=\sum_{i=1}^k a_i M_ib_i$ is a solution to the system of linear congruences: \begin{align*}
		X-a_i=\of{\sum_{j=1}^k a_j M_jb_j} - a_i=\sum_{\substack{j=1\\ j\neq i}}^k a_jM_jb_j + a_iM_ib_i-a_i
		&=\sum_{j=1,j\neq i}^k a_j M_jb_j + a_i(M_ib_i - 1)\\
		&\equiv\left[\sum_{j=1,j\neq i}^k a_j\cdot\of{\crossout[red]{0}{M_jb_j }}\right]+ a_i(M_ib_i - 1)\pmod{m_i}\quad\text{by (2)}\\
		&\equiv a_i\crossout[red]{0}{(M_ib_i - 1)}\quad\pmod{m_i}\quad\text{by (1)}\\
		&\equiv 0\pmod{m_i}.
	\end{align*}
	Therefore, we have:
	$$X-a_i \equiv 0 \pmod{m_i}$$
	Hence $X$ satisfies all of the linear congruence.\\
	\\
	(\textcolor{red}{Uniqueness}) Let $X_0,X_1$ are roots of the system of linear equations. Let $1\leq i\leq k$. Then \begin{align*}
		X_0\equiv &a_i\equiv X_1\pmod{m_i}
	\end{align*} and so \begin{align*}
		m_i&\mid X_0-X_1.
	\end{align*} Hence $m_1m_2\cdots m_k\mid X_0-X_1$, \ie, \[
	X_1\equiv X_2\pmod{M=m_1m_2\cdots m_k}.
	\]
\end{proof}
\vspace{4pt}
\section{Special Case of $\mathsf{CRT}$}

\iffalse
\begin{tcolorbox}[title=Chinese Remainder Theorem (CRT) - Special Case]
	\begin{theorem*}
		Given a system of $k$ linear congruences:
		\begin{align*}
			x&\equiv a_1 \pmod{m_1}\\
			x&\equiv a_2 \pmod{m_2}\\
			&\vdots \\
			x&\equiv a_k \pmod{m_k}
		\end{align*} where $m_1,m_2,\dots, m_k$ are pairwise coprime. Let $M=\prod_{i=1}^km_i$. Then, the unique solution of the system of congruences is give by \begin{align*}
			x&=\sum_{i=1}^ka_iM_ib_i\pmod{M}\\
			&=a_1M_1b_1+a_2M_2b_2+\cdots+a_kM_kb_k\pmod{M}.
		\end{align*} where $M_i=M/m_i$ and $ b_i\equiv\inv{M_i}\pmod{m_i}$.
	\end{theorem*}
\end{tcolorbox}\fi
\begin{tcolorbox}[colback=white,colframe=corcolor,arc=5pt,title={\color{white}\bf $\mathsf{CRT}$ - Special Case}]
	\begin{corollary*}
		Consider a system of two linear congruences:
		\begin{align*}
			x&\equiv a_1 \pmod{p}\\
			x&\equiv a_2 \pmod{q}
		\end{align*} where $p,q$ are coprime. Let $N=pq$. Then, the unique solution of the system of congruences is given by \begin{align*}
			\mathcolorbox{-green}{x=a_1qq_p^{-1}+a_2pp_q^{-1}\mod{N}}
		\end{align*} where $q_p^{-1}=\inv{q}\mod{p}$ and $p_{q}^{-1}=\inv{p}\mod{q}$.
	\end{corollary*}
\end{tcolorbox}
\iffalse
\begin{remark}
	Let $a,b\in\Z$ and $\gcd\of{a,b}=1$. Bézout's identity guarantees $\exists x,y\in\Z:ax+by=1$ and so \[
	ax+by=1\implies ax=(-y)b+1\implies ax\equiv1\pmod{b}.
	\] That is, \[
	\mathcolorbox{-blue}{\gcd\of{a,b}=1\implies\exists x\in\Z:ax\equiv1\pmod{b}}.
	\] Similarly, if $a$ and $b$ are coprime, $b$ has a mutiplicative inverse modulo $a$.
\end{remark}
\fi

\newpage
\begin{remark}\hypertarget{rmk1}{}
	Recall that \hyperlink{lem}{Bézout's identity} : $
	a,b\in\mathbb{Z}\implies\exists x,y\in\mathbb{Z}:\gcd(a,b)=ax+by.
	$ Especially, \[
	\text{$p,q$ are coprime}\implies\exists x,y\in\mathbb{Z}: px+qy=1.
	\] Since $p,q$ are coprime, we know that $\exists x,y\in\mathbb{Z}:px+qy=1$ and so \[
	px=(-y)q+1\quad\implies\quad px\equiv1\pmod{q}\quad\implies\quad x=p^{-1}\mod{q}.
	\] Similarly, $y=q^{-1}\mod{p}$. Thus we have $px+qy=1\implies pp_{q}^{-1}+qq_{p}^{-1}=1$. Consequently, \begin{align*}
		\hypertarget{crt}{}\mathcolorbox{-green}{x=a_1qq_p^{-1}+a_2pp_q^{-1}\mod{N}} &\implies x=a_1qq_p^{-1}+a_2(1-qq_{p}^{-1})\mod{N}\\
		&\implies \mathcolorbox{-red}{x=(a_1-a_2)qq_p^{-1}+a_2\mod{N}}.
	\end{align*}
\end{remark}
\vspace{4pt}
\section{$\rsa$-$\mathsf{CRT}$ Algorithm}

\RestyleAlgo{ruled}
\SetKwComment{Comment}{/* }{ */}
\begin{algorithm}[H]
	\caption{$\mathsf{RSA}$-$\mathsf{CRT}$ Algorithm}
	\KwData{The security parameter $k$, a public key $(N,e)$, a ciphertext $\mathcal{C}$.}
	\KwResult{The plaintext message $\mathcal{M}$ corresponding to the ciphertext $\mathcal{C}$.}
	\vspace{4pt}
	\vspace{4pt}
	\SetKwFunction{KeyGen}{KeyGen}
	\SetKwProg{Fn}{Function}{:}{}
	\Comment{Key Generation}
	\Fn{\KeyGen$(1^k)$}{
		$p, q \gets$ random prime numbers of $k/2$ bits each \tcp*{Generate two primes}
		$N \gets pq$ \tcp*{Compute modulus}
		$\phi(N) \gets (p-1)(q-1)$ \tcp*{Compute Euler's phi function}
		$e \gets$ integer $e\in\of{1,\phi(N)}$ s.t. $\gcd(e, \phi(N)) = 1$ \tcp*{Choose encryption exponent}
		$d \gets$ integer $d\in\of{1,\phi(N)}$ s.t. $ed\equiv 1\pmod{\phi\of{N}}$ \tcp*{Compute decryption exponent}
		${d_p\leftarrow d \mod p-1}$ \tcp*{Compute decryption exponent for $p$}
		${d_q \leftarrow d \mod q-1}$ \tcp*{Compute decryption exponent for $q$}
		$q_{inv} \gets$ integer $q_{inv}\in(1, p-1)$ s.t. $qq_{inv}\equiv1 \pmod{p}$ \tcp*{Compute $q$ inverse modulo $p$}
		Set the $\rsa$ public key as $(N,e)$\;
		Set the $\rsa$ secret key as $(p,q,d_p,d_q,q_{inv})$\;
	}
	\textbf{End Function}\\
	\vspace{4pt}
	\vspace{4pt}
	\Comment{Encryption}
	\SetKwFunction{Enc}{Enc}
	\Fn{\Enc$(N,e,\mathcal{M})$}{
		$\mathcal{C}\gets\mathcal{M}^e\mod N$ \tcp*{Encrypt with $e$ and $N$}
	}
	\textbf{End Function}\\
	\vspace{4pt}
	\vspace{4pt}
	\Comment{Decryption}
	\SetKwFunction{Dec}{Dec}
	\Fn{\Dec$(\mathcal{C})$}{
		$m_1 \gets \mathcal{C}^{d_p} \mod p$ \tcp*{Decrypt with $d_p$ and $p$}
		$m_2 \gets \mathcal{C}^{d_q} \mod q$ \tcp*{Decrypt with $d_q$ and $q$}
		$m \leftarrow (m_1 - m_2)qq_{inv}+m_2\mod N$ \tcp*{{$\mathcolorbox{-red}{m=(m_1-m_2)qq_{inv}+m_2\mod N}$}}
		\KwRet{$m$}\;
	}
	\textbf{End Function}\\
	\vspace{2.5pt}
\end{algorithm}
\newpage
\begin{proof}[Proof of Decryption]
	Note that \begin{align*}
		ed\equiv 1\pmod{(p-1)(q-1)}&\implies\exists k\in\Z:ed=1+k(p-1)(q-1),\\
		d_p=d\mod p-1&\implies\exists k_p\in\Z: d=(p-1)k_p+d_p.
	\end{align*}
	\hypertarget{ref1}{}Consider $m_1:=\mathcal{C}^{d_p}\mod p$. From $\mathcal{C}=\mathcal{M}^e\mod pq$, we have \begin{align*}
		\mathcal{C}\equiv\mathcal{M}^e\pmod{pq} \Leftrightarrow pq\mid \mathcal{C}-\mathcal{M}^e&\Leftrightarrow \mathcal{C}-\mathcal{M}^e=k_{N}\cdot pq\ \text{for some $k_{N}\in\Z$}\\
		&\Leftrightarrow \mathcal{C}-\mathcal{M}^e=\of{k_{N}q}\cdot p\\
		&\Leftrightarrow {p\mid \mathcal{C}-\mathcal{M}^e}\\
		&\Leftrightarrow \mathcolorbox{-blue}{\mathcal{C}\equiv\mathcal{M}^e\pmod{p}}.
	\end{align*} Then \begin{align*}
		m_1=\mathcal{C}^{d_p}\mod p
		=\of{\mathcal{M}^e}^{d-(p-1)k_p}\mod p=\of{{\mathcal{M}^{ed}}}\cdot{\mathcal{M}^{-e(p-1)k_p}}\mod p.
	\end{align*} Clearly, either $\gcd\of{\mathcal{M},p}=1$ or
	$\gcd\of{\mathcal{M},p}\neq 1$:
	\begin{itemize}
		\item[] \begin{tcolorbox}[colback=white,colframe=black,arc=5pt,title={\color{white}\bf }]
			\textbf{(Case I)} Let $\gcd\of{\mathcal{M},p}=1$. By \textcolor{magenta}{Fermat's little theorem}, we get \[
			{\mathcal{M}^{-e(p-1)k_p}}=\of{\textcolor{magenta}{\mathcal{M}^{p-1}}}^{-ek_p}\textcolor{magenta}{\equiv} \textcolor{magenta}{1}^{-ek_p}=1\textcolor{magenta}{\pmod{p}}.
			\] Thus, \begin{align*}
				m_1=\mathcal{C}^{d_p}\mod p&=\of{{\mathcal{M}^{ed}}}\cdot\crossout[red]{1}{\mathcal{M}^{-e(p-1)k_p}}\mod p\quad\text{by FLT}\\
				&\equiv\mathcal{M}^{k(p-1)(q-1)+1}\pmod{p}\\
				&\equiv\of{\crossout[red]{1}{\mathcal{M}^{p-1}}}^{k(q-1)}\cdot\mathcal{M}\pmod{p}\quad\text{by FLT}\\
				&\equiv\mathcal{M}\pmod{p}.
			\end{align*} That is, $m_1\equiv\mathcal{M}\pmod{p}$.
		\end{tcolorbox}
		\item[] \begin{tcolorbox}[colback=white,colframe=black,arc=5pt,title={\color{white}\bf }]
			\textbf{(Case II)} Let $\gcd\of{\mathcal{M},p}\neq 1$, \ie, $\exists l\in\Z:\mathcal{M}=pl$ since $p$ is a primes\footnote{Since $p$ is a prime, $p$ has factors $1$ and $p$ only. Then $\gcd\of{\mathcal{M},p}\neq 1$ means that $p$ is only common factor.}. Then we have \[
			\mathcal{M}=pl\implies p\mid\mathcal{M}-0\implies\mathcal{M}\equiv 0\pmod{p}.
			\] Recall that {$\mathcolorbox{-blue}{\mathcal{C}\equiv\mathcal{M}^e\pmod{p}}$}. Then $\mathcal{C}\equiv\mathcal{M}^e\equiv 0^e=0\pmod{p}$ and so\[
			m_1=\mathcal{C}^{d_p}\mod p=0^{d_p}\mod p= 0\mod p=0.
			\] That is, $m_1\equiv 0\pmod{p}$. Therefore \[
			\begin{cases}
				\mathcal{M}\equiv 0\pmod{p}\\
				m_1\equiv 0\pmod{p}
			\end{cases}\implies m_1\equiv\mathcal{M}\pmod{p}.
			\] 
		\end{tcolorbox}
	\end{itemize} 
	Here, we obtain $m_1\equiv\mathcal{M}\pmod{p}$. Similarly, we have $m_2\equiv\mathcal{M}\pmod{q}$. Then, the plaintext message $\mathcal{M}$ is a solution to the following system of two linear congruences: \begin{align*}
		\mathcal{M}&\equiv m_1\pmod{p},\\
		\mathcal{M}&\equiv m_2\pmod{q}.
	\end{align*}
	Then, \hyperlink{rmk1}{\textbf{Remark 1}} guarantees that \[
	\mathcal{M}=(m_1-m_2)qq_{inv}+m_2\mod pq.
	\]
\end{proof}

\footer{Department of Information Security, Cryptography and Mathematics, Kookmin University}
\end{document}
