\documentclass{article}

% Packages for formatting
\usepackage[margin=1in]{geometry}
\usepackage{fancyhdr}
\usepackage{enumerate}
\usepackage{graphicx}
\usepackage{kotex}
\usepackage{amsmath}
\usepackage{amsthm}
\usepackage{algorithm2e,setspace}
\usepackage{algpseudocode}
\usepackage{xcolor}
\usepackage{amssymb}

% Fonts
\usepackage[T1]{fontenc}
\usepackage[utf8]{inputenc}
\usepackage{newpxtext,newpxmath}
\usepackage{sectsty}

% Define colors
\definecolor{blue1}{HTML}{0077c2}
\definecolor{blue2}{HTML}{00a5e6}
\definecolor{blue3}{HTML}{b3e0ff}
\definecolor{blue4}{HTML}{00293c}
\definecolor{blue5}{HTML}{e6f7ff}

\definecolor{thmcolor}{RGB}{231, 76, 60}
\definecolor{defcolor}{RGB}{52, 152, 219}
\definecolor{lemcolor}{RGB}{155, 89, 182}
\definecolor{corcolor}{RGB}{46, 204, 113}
\definecolor{procolor}{RGB}{241, 196, 15}

\usepackage{color,soul}
\usepackage{soul}
\newcommand{\mathcolorbox}[2]{\colorbox{#1}{$\displaystyle #2$}}
\usepackage{cancel}
\newcommand\crossout[3][black]{\renewcommand\CancelColor{\color{#1}}\cancelto{#2}{#3}}
\newcommand\ncrossout[2][black]{\renewcommand\CancelColor{\color{#1}}\cancel{#2}}

\usepackage{hyperref}
\usepackage{booktabs}

% Chapter formatting
\definecolor{titleblue}{RGB}{0,53,128}
\usepackage{titlesec}
\titleformat{\section}
{\normalfont\sffamily\Large\bfseries\color{titleblue!100!gray}}{\thesection}{1em}{}
\titleformat{\subsection}
{\normalfont\sffamily\large\bfseries\color{titleblue!50!gray}}{\thesubsection}{1em}{}

%Tcolorbox
\usepackage[most]{tcolorbox}

%Tikzpicture
\usepackage{pgfplots}
\usepgfplotslibrary{polar}
%\pgfplotsset{compat=1.17}
\usepackage{tikz-cd}
\usetikzlibrary{positioning}
\usetikzlibrary{angles, quotes}

% Header and footer formatting
\pagestyle{fancy}
\fancyhead{}
\fancyhf{}
\rhead{Student ID: 20192250\quad Name: 지용현}%\rule{3cm}{0.4pt}}
\lhead{\textcolor{blue2}{\textbf{CA\hspace{4pt} 2023-spring-Final}}}
% Define footer
\newcommand{\footer}[1]{
\begin{flushright}
	\vspace{2em}
	\includegraphics[width=2cm]{school_logo.jpg} \\
	\vspace{1em}
	\textcolor{blue2}{\small\textbf{#1}}
\end{flushright}
}
%\rfoot{\large Department of Information Security, Cryptogrphy and Mathematics, Kookmin Uni.\includegraphics[height=1.5cm]{school_logo.jpg}}
\fancyfoot{}
\fancyfoot[C]{-\thepage-}

\usepackage{pifont}

\newcommand{\ie}{\textnormal{i.e.}}
\newcommand{\rsa}{\mathsf{RSA}}
\newcommand{\rsacrt}{\mathsf{RSA}\textendash\mathsf{CRT}}
\newcommand{\inv}[1]{#1^{-1}}

\usepackage{amsthm}
\newtheorem{axiom}{Axiom}[section]
\newtheorem{theorem}{Theorem}
\newtheorem*{theorem*}{Theorem}
\newtheorem{proposition}[theorem]{Proposition}
\newtheorem{corollary}{Corollary}[theorem]
\newtheorem*{corollary*}{Corollary}
\newtheorem{lemma}[theorem]{Lemma}
\newtheorem*{lemma*}{Lemma}

\theoremstyle{definition}
\newtheorem{definition}{Definition}
\newtheorem*{definition*}{Definition}
\newtheorem{remark}{Remark}
\newtheorem{exercise}{Exercise}[section]

%New Command
\newcommand{\set}[1]{\left\{#1\right\}}
\newcommand{\N}{\mathbb{N}}
\newcommand{\Z}{\mathbb{Z}}
\newcommand{\Q}{\mathbb{Q}}
\newcommand{\R}{\mathbb{R}}
\newcommand{\C}{\mathbb{C}}
\newcommand{\F}{\mathbb{F}}
\newcommand{\nbhd}{\mathcal{N}}
\newcommand{\Log}{\operatorname{Log}}
\newcommand{\Arg}{\operatorname{Arg}}
\newcommand{\pv}{\operatorname{P.V.}}

\newcommand{\of}[1]{\left( #1 \right)} 
\newcommand{\abs}[1]{\left\lvert #1 \right\rvert}
\newcommand{\norm}[1]{\left\| #1 \right\|}

\newcommand{\sol}{\textcolor{magenta}{\bf Sol}}
\newcommand{\conjugate}[1]{\overline{#1}}
\newcommand{\res}{\operatorname{res}}
\newcommand{\Res}{\operatorname{Res}}

\renewcommand{\Re}{\operatorname{Re}}
\renewcommand{\Im}{\operatorname{Im}}

\begin{document}
\pagenumbering{arabic}
\begin{center}
	\huge\textbf{Complex Analysis - Final}\\
	\vspace{0.5em}
\end{center}

\begin{tcolorbox}[colback=white,colframe=white,arc=5pt,title={\color{black}\bf $\bullet$ Radius of Convergence}]
	Determine the radius of convergence for the following infinite series of complex terms. \[
	\text{(1)}\ \sum_{n=1}^{\infty}\frac{1}{3^n}(z-i)^n\quad\quad\quad\quad\quad\quad\quad\quad\quad\quad
	\text{(2)}\ \sum_{n=1}^{\infty}\frac{1}{n}z^n
	\]
\end{tcolorbox}
\begin{proof}[\sol]
	\begin{enumerate}[(1)]
		\item Let $a_n=1/3^n$ then $\displaystyle
		R=\lim\limits_{n\to\infty}\frac{\abs{a_n}}{\abs{a_{n+1}}}=\lim\limits_{n\to\infty}\frac{\abs{1/3^n}}{\abs{1/3^{n+1}}}=\lim\limits_{n\to\infty}\left[\frac{1}{3^n}\cdot 3^{n+1}\right]=3.$
		\item Let $a_n=1/n$ then $\displaystyle
		R=\lim\limits_{n\to\infty}\frac{\abs{1/n}}{\abs{1/n+1}}=\lim\limits_{n\to\infty}\left[\frac{1}{n}\cdot (n+1)\right]=\lim\limits_{n\to\infty}=\lim\limits_{n\to\infty}\of{\frac{1}{n}+1}=1.$
	\end{enumerate}
\end{proof}
\begin{tcolorbox}[colback=white,colframe=black,arc=5pt,title={\color{white}\bf Taylor Series}]
	If $f$ is entire function, then $\displaystyle
	f(z)=\sum_{n=0}^{\infty}\frac{f^{(n)}(z_0)}{n!}(z-z_0)^n
	$ for some $z_0\in\C$.
\end{tcolorbox}
\begin{tcolorbox}[colback=white,colframe=black,arc=5pt,title={\color{white}\bf Maclaurin's Series}]
	\begin{itemize}
		\item $\displaystyle e^z=\sum_{n=0}^{\infty}\frac{1}{n!}z^n=1+z+\frac{1}{2!}z^2+\frac{1}{3!}z^3+\cdots$\quad $(\forall z\in\C)$
		\item $\displaystyle
		\sin z=\sum_{n=0}^{\infty}\frac{(-1)^n}{(2n+1)!}z^{2n+1}=z-\frac{1}{3!}z^3+\frac{1}{5!}z^5-\cdots$\quad $(\forall z\in\C)$
		\item $\displaystyle
		\cos z=\sum_{n=0}^{\infty}\frac{(-1)^n}{(2n)!}z^{2n}=1-\frac{1}{2!}z^2+\frac{1}{4!}z^4-\cdots$\quad $(\forall z\in\C)$
	\end{itemize}
\end{tcolorbox}
\begin{tcolorbox}[colback=white,colframe=white,arc=5pt,title={\color{black}\bf $\bullet$ Series Expansion of a Complex Function I}]
	\begin{enumerate}[(1)]
		\item What is the coefficient of $z^3$ when the complex function $\displaystyle f=\frac{1}{(z-1)^2}$ is expanded into a series centered at $z_0=0$?
		\item When expanding the complex function $\displaystyle f(z)=\frac{5z-2}{z(z-1)}$ into a series centered at $z_0=0$, let the coefficient of $\inv{z}$ be $a$, and when expanding it into a series centered at $z=1$, let the coefficient of $(z-1)^{-1}$ be b. Then, what is $a+b$?
		\item What is the coefficient of $z^{-1}$ when the complex function $\displaystyle f=\frac{\sin z-z}{z^3}$ is expanded into a series centered at $z_0=0$?
		\item What is the coefficient of $z^{-2}$ when the complex function $\displaystyle f=\frac{z^3-1}{\sin(z^2)}$ is expanded into a series centered at $z_0=0$?
	\end{enumerate}
\end{tcolorbox}
\begin{proof}[\sol]
	\begin{enumerate}[(1)]
		\item $f(z)=1/(z-1)^2$ is holomorphic in $B_1(0)=\set{z\in\C:\abs{z-0}<1}$. Since \begin{align*}
			f^{(0)}&=(z-1)^{-2},\\
			f^{(1)}&=-2(z-1)^{-3},\\
			f^{(2)}&=(-2)(-3)(z-1)^{-4},\\
			&\vdots\\
			f^{(n)}&=\frac{(-1)^n(n+1)!}{(z-1)^{n+2}},
		\end{align*} we have $f^{(n)}(0)=(n+1)!$. Thus \[
		f(z)=\sum_{n=0}^{\infty}\frac{f^{(n)}(0)}{n!}(z-0)^n=\sum_{n=0}^\infty \frac{(n+1)!}{n!}z^n=\sum_{n=0}^\infty (n+1)z^n\quad(\abs{z}<1).
		\] Hence, the coefficient of $z^3$ is $4$.
		\vspace{4pt}
		\item \begin{enumerate}[(i)]
			\item $(z_0=0)$; $\displaystyle f(z)=\frac{5z-2}{z(z-1)}$ is holomorphic in $B_1^*(0)=\set{z\in\C:0<\abs{z-0}<1}$. \begin{align*}
				f(z)=\frac{5z-2}{z(z-1)}&=\frac{2-5z}{z}\cdot\frac{1}{1-z}\\
				&=\of{\frac{2}{z}-5}\of{1+z+z^2+z^3+\cdots}\quad(\abs{z}<1)\\
				&=\frac{2}{z}+2+2z+2z^2+\cdots\\
				&\hspace{7mm}-5-5z-5z^2-\cdots\\
				&=\frac{2}{z}-3-3z-3z^2-\cdots\\
				&=2z^{-1}+\sum_{n=0}^{\infty}(-3)z^n.
			\end{align*}
			Thus, the coefficient of $z^{-1}$ is $a=2$.
			\item $(z_0=1)$; $f$ is holomorphic in $B_1^*(1)=\set{z\in\C:0<\abs{z-1}<1}$. Let $w:=z-1$, \ie, $0<\abs{w}<1$ then \begin{align*}
				f(z)=\frac{5z-2}{z(z-1)}&=\frac{5(w+1)-2}{(w+1)w}\quad(w\notin\set{-1,0})\\
				&=\frac{1}{w+1}\cdot\frac{5w+3}{w}\\
				&=\frac{1}{1-(-w)}\cdot\of{\frac{3}{w}+5}\\
				&=\of{1+(-w)+(-w)^2+(-w)^3+\cdots}\of{\frac{3}{w}+5}\\
				&=\frac{3}{w}-3+3w-3w^2+3w^3-\cdots\\
				&\hspace{8mm}+5-5w+5w^2-5w^3+\cdots\\
				&=3\inv{w}+2-2w+2w^2-2w^3+\cdots\\
				&=3w^{-1}+\sum_{n=0}^\infty (-1)^n2w^n\\
				&=3(z-1)^{-1}+\sum_{n=0}^\infty (-1)^n2(z-1)^n.
			\end{align*} Thus, the coefficient of $(z-1)^{-1}$ is $b=3$.
		\end{enumerate}
		Hence, by (i) and (ii), $a+b=5$.
		\vspace{4pt}
		\item \begin{align*}
			f(z)=\frac{\sin z-z}{z^3}&=\frac{1}{z^3}\left[\of{z-\frac{1}{3!}z^3+\frac{1}{5!}z^5-\cdots}-z\right]\\
			&=\frac{1}{z^3}\of{-\frac{1}{3!}z^3+\frac{1}{5!}z^5-\frac{1}{7!}z^7+\cdots}\\
			&=-\frac{1}{3!}+\frac{1}{5!}z^2-\frac{1}{7!}z^4+\cdots\\
			&=\sum_{n=0}^\infty(-1)^{n+1}\frac{1}{(2n+3)!}z^{2n}.
		\end{align*}
		Thus, the coefficient of $z^{-1}$ is $0$.
		\vspace{4pt}
		\item Let $z\neq 0$. \begin{align*}
			f(z)=\frac{z^3-1}{\sin(z^2)}&=(z^3-1)\cdot\frac{1}{\displaystyle z^2-\frac{1}{3!}(z^2)^3+\frac{1}{5!}(z^2)^5-\frac{1}{7!}(z^2)^7+\cdots}\\
			&=\of{z-\frac{1}{z^2}}\left[1-\frac{1}{3!}z^4+\frac{1}{5!}z^8-\frac{1}{7!}z^{12}+\cdots\right]^{-1}\\
			&=\of{z-\frac{1}{z^2}}\left[1+\of{\frac{1}{3!}z^4-\frac{1}{5!}z^8+\frac{1}{7!}z^{12}-\cdots}\right]^{-1}\\
			&=\of{z-\frac{1}{z^2}}\of{1+\phi(z)+\phi(z)^2+\cdots}\quad\text{with}\quad\phi(z)=\sum_{n=0}^\infty\frac{(-1)^{n}}{(2n+3)!}z^{4(n+1)}.
		\end{align*}
		Thus, the coefficient of $z^{-2}$ is $-1$.
	\end{enumerate}
\end{proof}

\begin{tcolorbox}[colback=white,colframe=white,arc=5pt,title={\color{black}\bf $\bullet$ Series Expansion of a Complex Function II}]
	Expand the following complex function $f(z)$ into a power series centered at the given $z_0$. \begin{enumerate}[(1)]
		\item $\displaystyle f(z)=\frac{1}{z^2+1}$,\quad $z_0=i$.
		\item $\displaystyle f(z)=\frac{e^z}{1-z}$,\quad $z_0=0$.
		\item $\displaystyle f(z)=z\cos\of{\frac{1}{z}}$,\quad $z_0=0$.
	\end{enumerate}
\end{tcolorbox}
\begin{proof}[\sol]
	\begin{enumerate}[(1)]
		\item $f$ is holomorphic in $B_2^*(i)=\set{z\in\C:0<\abs{z-i}<2}$.
		\begin{center}
			\begin{tikzpicture}[scale=.75]
				\draw[->] (-3.25,0) -- (3,0) node[right] {$\operatorname{Re}(z)$};
				\draw[->] (0,-1.25) -- (0,3.25) node[above] {$\operatorname{Im}(z)$};
				\draw[dashed,thick,red] (2,1) arc (0:360:2) node[above right] {$B_2^*(i)$};
				\node[below left] at (0,0) {$O$};
				\node[above left, red] at (0,1) {$i$};
				\node[above left, red] at (0,-1) {$-i$};
				\draw[fill=black] ({sqrt(3)},0) circle (0.05) node[below] {$\sqrt{3}$};
				\draw[fill=black] (-{sqrt(3)},0) circle (0.05) node[below] {$-\sqrt{3}$};
				\draw[red, mark size=5pt] plot[mark=x] coordinates{(0,1)};
				\draw[red, mark size=5pt] plot[mark=x] coordinates{(0,-1)};
				\draw[red] (0,1) -- (2,1) node[midway, above] {$2$};
			\end{tikzpicture}
		\end{center} Note that $0<\abs{z-i}<2\implies 0<\displaystyle\frac{\abs{z-i}}{2}<1$.
		\begin{align*}
			f(z)=\frac{1}{z^2+1}&=\frac{1}{z-i}\cdot\frac{1}{z+i}\\
			&=\frac{1}{z-i}\cdot\frac{1}{2i+z-i}\\
			&=\frac{1}{z-i}\cdot\frac{1/2i}{1-\of{-\displaystyle\frac{z-i}{2i}}}\\
			&=\frac{1}{z-i}\cdot\frac{1}{2i}\cdot\left[1+\of{\frac{z-i}{-2i}}+\of{\frac{z-i}{-2i}}^2+\of{\frac{z-i}{-2i}}^3+\cdots\right]\quad\because\abs{\frac{z-i}{-2i}}=\frac{\abs{z-i}}{2}<1\\
			&=\frac{1}{2i}(z-i)^{-1}+\frac{1}{2i(-2i)}+\frac{1}{2i(-2i)^2}(z-i)+\frac{1}{2i(-2i)^3}(z-i)^2+\cdots\\
			&=\frac{1}{2i}(z-i)^{-1}+\sum_{n=0}^\infty\frac{(-1)^{n+1}}{(2i)^{n+2}}(z-i)^n.
		\end{align*}
		\item Let $\abs{z}<1$ then \begin{align*}
			f(z)=\frac{e^z}{1-z}&=\of{1+z+\frac{1}{2!}z^2+\frac{1}{3!}z^3+\cdots}\of{1+z+z^2+z^3+\cdots}\\
			&=1+z+\frac{1}{2!}z^2+\frac{1}{3!}z^3+\frac{1}{4!}z^4+\cdots\\
			&\hspace{6mm}+z+z^2+\frac{1}{2!}z^3+\frac{1}{3!}z^4+\cdots\\
			&\hspace{12mm}+z^2+z^3+\frac{1}{2!}z^4+\cdots\\
			&=\frac{1}{0!}+\of{\frac{1}{1!}+\frac{1}{0!}}z+\of{\frac{1}{2!}+\frac{1}{1!}+\frac{1}{0!}}z^2+\of{\frac{1}{3!}+\frac{1}{2!}+\frac{1}{1!}+\frac{1}{0!}}z^3+\cdots\\
			&=\sum_{n=0}^\infty\of{\sum_{k=0}^n\frac{1.}{k!}z^n}.
		\end{align*}
		\item Let $z\neq 0$ then \begin{align*}
			f(z) = z\cos\of{\frac{1}{z}}&=z\cdot\left[1-\frac{1}{2!}\of{\frac{1}{z}}^2+\frac{1}{4!}\of{\frac{1}{z}}^4-\frac{1}{6!}\of{\frac{1}{z}}^6+\cdots\right]\\
			&=z-\frac{1}{2!}\of{\frac{1}{z}}+\frac{1}{4!}\of{\frac{1}{z}}^3-\frac{1}{6!}\of{\frac{1}{z}}^5+\cdots\\
			&=\sum_{n=0}^\infty\frac{(-1)^n}{(2n)!}z^{-(2n-1)}.
		\end{align*}
	\end{enumerate}
\end{proof}
\vspace{8pt}

\begin{tcolorbox}[colback=white,colframe=white,arc=5pt,title={\color{black}\bf $\bullet$ Series Expansion of a Complex Function III}]
	Represent the function \[
	f(z)=\frac{1}{(z-1)(z-2)}
	\] in the form of $\sum_{n=-\infty}^\infty c_n(z-z_0)^n$ in each of the following regions with respect to the given $z_0$.
	\begin{enumerate}
		\item[(1)] $0<\abs{z-1}<1$,\quad $z_0=1$\hspace{24mm} (2) $1<\abs{z}<2$,\quad $z_0=0$
		\item[(3)] $\abs{z}<1$,\quad $z_0=0$\hspace{36mm} (4) $\abs{z}>2$,\quad $z_0=0$
	\end{enumerate}
	\begin{center}
		\begin{tikzpicture}[scale=1.2]
			\draw[->] (-3.25,0) -- (3,0) node[right] {$\operatorname{Re}(z)$};
			\draw[->] (0,-1.25) -- (0,3.25) node[above] {$\operatorname{Im}(z)$};
			\foreach \i in {-4,...,-2,-1,1,2,...,4}
			\draw[] (\i,.1)--(\i,-.1) node[below] {$\i$};
			\foreach \i in {-1,1,2}
			\draw[] (.1,\i)--(-.1,\i) node[left] {$\i i$};
			\draw[dashed,thick,blue] (2,0) arc (0:360:1) node[above right] {$(1)$};
			%\node[below left] at (0,0) {$O$};
			%\draw[fill=black] ({sqrt(3)},0) circle (0.05) node[below] {$\sqrt{3}$};
			%\draw[fill=black] (-{sqrt(3)},0) circle (0.05) node[below] {$-\sqrt{3}$};
			\draw[red, mark size=2.5pt] plot[mark=x] coordinates{(1,0)} node[] {};
			\draw[red, mark size=2.5pt] plot[mark=x] coordinates{(2,0)} node[] {};
			%\node[above left, red] at (1,0) {$1$};
			%\node[above left, red] at (2,0) {$2$};
			%\draw[red] (0,1) -- (2,1) node[midway, above] {$2$};
		\end{tikzpicture}
	\end{center}
\end{tcolorbox}
\begin{proof}[\sol]
	\begin{enumerate}[(1)]
		\item \begin{align*}
			f(z)=\frac{1}{z-1}\cdot\frac{1}{z-2}&=\frac{1}{z-1}\cdot\frac{-1}{1-(z-1)}\\
			&=\frac{-1}{z-1}\of{1+(z-1)+(z-1)^2+\cdots}\quad\because\abs{z-1}<1\\
			&=-(z-1)^{-1}+(-1)+(-1)(z-1)+(-1)(z-1)^2+\cdots\\
			&=-(z-1)^{-1}+\sum_{n=0}^\infty(-1)(z-1)^n.
		\end{align*}
		\item Note that $\displaystyle f(z)=\frac{-1}{z-1}+\frac{1}{z-2}$. Then \[
		\begin{cases}
			\frac{-1}{z-1}=\frac{-1/z}{1-1/z}=-\frac{1}{z}\of{1+\of{\frac{1}{z}}+\of{\frac{1}{z}}^2+\cdots} &\because\abs{z}>1,\\
			\\
			\frac{1}{z-2}=\frac{-1/2}{1-z/2}=-\frac{1}{2}\of{1+\of{\frac{z}{2}}+\of{\frac{z}{2}}^2+\cdots} &\because\abs{z}<2.
		\end{cases}
		\] Thus \begin{align*}
			f(z)&=\of{-\frac{1}{z}-\frac{1}{z^2}-\frac{1}{z^3}-\cdots}+\of{-\frac{1}{2}-\frac{z}{2^2}-\frac{z^2}{2^3}+\cdots}=\sum_{n=1}^\infty(-1)z^{-n}+\sum_{n=0}^\infty\frac{-1}{2^{n+1}}z^n.
		\end{align*}
		\item Note that $\displaystyle f(z)=\frac{-1}{z-1}+\frac{1}{z-2}$. Then \[
		\begin{cases}
			\frac{-1}{z-1}=\frac{1}{1-z}=1+z+z^2+z^3+\cdots &\because\abs{z}<1,\\
			\\
			\frac{1}{z-2}=\frac{-1/2}{1-z/2}=-\frac{1}{2}\of{1+\of{\frac{z}{2}}+\of{\frac{z}{2}}^2+\cdots} &\because\abs{\frac{z}{2}}<\frac{1}{2}<1.
		\end{cases}
		\] Thus \begin{align*}
			f(z)&=\of{1+z+z^2+z^3+\cdots}+\of{-\frac{1}{2}-\frac{z}{2^2}-\frac{z^2}{2^3}-\cdots}\\
			&=\of{1-\frac{1}{2}}+\of{1-\frac{1}{2^2}}z+\of{1-\frac{1}{2^3}}z^2+\cdots\\
			&=\sum_{n=0}^\infty\of{1-\frac{1}{2^{n+1}}}z^n.
		\end{align*}
		\item Note that $\displaystyle f(z)=\frac{-1}{z-1}+\frac{1}{z-2}$. Then \[
		\begin{cases}
			\frac{-1}{z-1}=\frac{-1/z}{1-1/z}=-\frac{1}{z}\of{1+\of{\frac{1}{z}}+\of{\frac{1}{z}}^2+\cdots} &\because\abs{\frac{1}{z}}<\frac{1}{2}<1,\\
			\\
			\frac{1}{z-2}=\frac{1/z}{1-2/z}=\frac{1}{z}\of{1+\of{\frac{2}{z}}+\of{\frac{2}{z}}^2+\cdots} &\because\abs{\frac{2}{z}}<1.
		\end{cases}
		\] Thus \begin{align*}
			f(z)&=\of{-\frac{1}{z}-\frac{1}{z^2}-\frac{1}{z^3}-\cdots}+\of{\frac{1}{z}+\frac{2}{z^2}+\frac{2^2}{z^3}+\cdots}\\
			&=(-1+2^0)z^{-1}+(-1+2^1)z^{-2}+(-1+2^2)z^{-3}+\cdots\\
			&=\sum_{n=0}^\infty\of{2^n-1}z^{-(n+1)}.
		\end{align*}
	\end{enumerate}
\end{proof}

\begin{tcolorbox}[colback=white,colframe=white,arc=5pt,title={\color{black}\bf $\bullet$ Residue}]
	Find $\displaystyle \res\left[\frac{2z+4}{z^2-1},1\right]$. 
\end{tcolorbox}
\begin{proof}[\sol]
	Consider $0<\abs{z-1}<2$. \begin{align*}
		\frac{2z+4}{z^2-1}&=\frac{2z+4}{(z-1)(z+2)}\\
		&=\frac{2w+6}{w(w+2)}\quad w:=z-1,\ \ie,\ 0<\abs{w}<2 \\
		&=\of{\frac{2w+6}{w}}\cdot\of{\frac{1}{2-(-w)}}\\
		&=\of{2+\frac{6}{w}}\cdot\of{\frac{1/2}{1-(-w/2)}}\\
		&=\of{2+\frac{6}{w}}\cdot\frac{1}{2}\cdot\of{1+(-w/2)+(-w/2)^2+\cdots}\quad\because\abs{\frac{w}{2}}<1\\
		&=\of{1+\frac{3}{w}}\of{1+(-w/2)+(-w/2)^2+\cdots}\\
		&=\cdots+3w^{-1}+\cdots\\
		&=\cdots+3(z-1)^{-1}+\cdots.
	\end{align*}
	Thus $\displaystyle\res\left[\frac{2z+4}{z^2-1},1\right]=3.$
\end{proof}
\vspace{8pt}
\begin{tcolorbox}[colback=white,colframe=black,arc=5pt,title={\color{white}\bf Classification of Singularities}]
	\begin{enumerate}[(1)]
		\item Let $f:D\to\C$. $z_0\in\C$ is \[
		\begin{cases}
			\text{Analystic Point}\\
			\\
			\text{Singularity}\begin{cases}
				\text{Isolated Singularity}
				\begin{cases}
					\text{Removable Singularity}\iff\exists\lim\limits_{z\to z_0} f(z)\\
					\\
					\text{Pole of order $k\geq 1$}\iff\exists\lim\limits_{z\to z_0}(z-z_0)^kf(z)\neq 0\\
					\\
					\text{Essential Singularity}
				\end{cases}
				\\
				\\
				\text{Non-isolated Singularity}
			\end{cases}
		\end{cases}
		\]
		\item The classification order of isolated singularities: \[
		\text{Isolated Singularity}?\longrightarrow\text{Removable Singularity}?\longrightarrow\text{Pole of Order $k$}?\longrightarrow\text{Essential Singularity}?.
		\]
	\end{enumerate}
\end{tcolorbox}

\begin{tcolorbox}[colback=white,colframe=white,arc=5pt,title={\color{black}\bf $\bullet$ Classification of Singularities I}]
	Classify the singularity at the isolated singularity $z_0$ of the following function $f$:
	\begin{enumerate}[(1)]
		\item $\displaystyle f(z)=\frac{\sin^2z}{z^2\cos z}$,\quad $z_0=0$
		\item $\displaystyle f(z)=\frac{1-e^{z^2}}{\sin^2z\cos z}$,\quad $z_0=0$
		\item $\displaystyle f(z)=\frac{\cos z-1}{z^2\sin z}$,\quad $z_0=0$
		\item $\displaystyle f(z)=\frac{z^3e^z}{z^{10}-1}$,\quad $z_0=1$
		\item $\displaystyle f(z)=\frac{\sin z\cos z}{z^4}$,\quad $z_0=0$
		\item $\displaystyle f(z)=e^{\displaystyle\frac{1+2z}{z}}$,\quad $z_0=0$
	\end{enumerate}
\end{tcolorbox}
\begin{proof}[\sol]
	\begin{enumerate}[(1)]
		\item \[
		\lim\limits_{z\to 0}f(z)=\lim\limits_{z\to 0}\left[\of{\frac{\sin z}{z}}^2\frac{1}{\cos z}\right]=1.
		\] Thus $z_0=0$ is a removable singularity.
		\item \begin{align*}
			\lim\limits_{z\to 0}\frac{1-e^{z^2}}{\sin^2z\cos z}&=\lim\limits_{z\to 0}\frac{1-e^{z^2}}{\sin^2z}\\
			&=\lim\limits_{z\to 0}\frac{-2ze^{z^2}}{2\sin z\cos z}\quad\text{by L'Hôpital's rule}\\
			&=\lim\limits_{z\to 0}\left[-\of{\frac{1}{\sin z/z}}\cdot\frac{e^{z^2}}{\cos z}\right]\\
			&=-1.
		\end{align*}
		Thus $z_0=0$ is a removable singularity.
		\item \begin{align*}
			\lim\limits_{z\to 0}zf(z)=\lim\limits_{z\to 0}\frac{\cos z-1}{z\sin z}&=\lim\limits_{z\to 0}\frac{-\sin z}{\sin z+z\cos z}\\
			&=\lim\limits_{z\to 0}\frac{-\cos z}{\cos z+\cos z-z\sin z}\\
			&=-\frac{1}{2}\neq 0.
		\end{align*} Thus $z_0=0$ is a simple pole.
		\item \begin{align*}
			\lim\limits_{z\to 1}(z-1)f(z)=\lim\limits_{z\to 1}\frac{(z^4-z^3)e^z}{z^{10}-1}&=\lim\limits_{z\to 1}\frac{(z^4-z^3)e^z+(4z^3-3z^2)e^z}{10z^{9}}\\
			&=\frac{e}{10}\neq 0.
		\end{align*} Thus $z_0=1$ is a simple pole.
		\item \[
		\lim\limits_{z\to 0}z^3f(z)=\lim\limits_{z\to 0}\left[\of{\frac{\sin z}{z}}{\cos z}\right]=1\neq 0.
		\] Thus $z_0=0$ is a pole of order $3$.
		\item Note that \[
		\lim\limits_{\substack{x\to 0+\\ y=0}}e^{1/z}=\lim\limits_{x\to 0+}e^{1/x}=\infty\neq 0=\lim\limits_{x\to 0-}e^{1/x}=\lim\limits_{\substack{x\to 0-\\ y=0}}e^{1/z},
		\] and so $\not\exists\lim\limits_{z\to 0}e^{1/z}$. We claim that
		$\forall k\in\Z^+:\not\exists\lim\limits_{z\to 0} z^ke^{\frac{1}{z}}:$ let $k\in\Z^+$ then
		\begin{align*}
			\lim\limits_{\substack{x\to 0+\\ y=0}}z^ke^{1/z}&=\lim\limits_{\substack{x\to 0+\\ y=0}}z^k\left[1+\of{\frac{1}{z}}+\frac{1}{2!}\of{\frac{1}{z}}^2+\cdots\right]\\
			&=\lim\limits_{x\to 0+}x^k\left[1+\of{\frac{1}{x}}+\frac{1}{2!}\of{\frac{1}{x}}^2+\cdots\right]\\
			&\geq\lim\limits_{x\to 0+}\frac{x^k}{(k+1)!x^{k+1}}=\frac{1}{(k+1)!}\lim\limits_{x\to 0+}\frac{1}{x}=\infty.
		\end{align*} Thus $z_0=0$ is an essential singularity.
	\end{enumerate}
\end{proof}
\vspace{8pt}
\begin{tcolorbox}[colback=white,colframe=white,arc=5pt,title={\color{black}\bf $\bullet$ Classification of Singularities II}]
	Find and classify all singularities of the following complex function.
	\begin{enumerate}[(1)]
		\item $\displaystyle f(z)=\frac{\cos z}{z^2}$
		\item $\displaystyle f(z)=\frac{z^2+3z-1}{z+2}$
		\item $\displaystyle f(z)=\frac{e^z}{(z-1)^3}$
		\item $\displaystyle f(z)=\frac{z+1}{(z^2+4)(z-1)^3}$
	\end{enumerate}
\end{tcolorbox}
\begin{proof}[\sol]
	\begin{enumerate}[(1)]
		\item The singularity is at $0$ and it is a pole of order $2$.
		\item The singularity is at $-2$ and it is a pole of order $1$ (that is, simple pole).
		\item The singularity is at $1$ and it is a pole of order $3$.
		\item The singularities are at $2i$, $-2i$, and $1$, each of which is a pole with orders $1$, $1$, and $3$, respectively.
	\end{enumerate}
\end{proof}
\vspace{8pt}
\begin{tcolorbox}[colback=white,colframe=white,arc=5pt,title={\color{black}\bf \textcolor{red}{$\star$} Classification of Singularities III}]
	Let's assume the complex function $f:\C\setminus\set{0}\to\C$ is analytic in $\C\setminus\set{0}$ and it satisfies \[
	\abs{f(z)}\leq\abs{z}+\frac{1}{\sqrt{\abs{z}}}\quad(\forall z\in\C\setminus\set{0}).
	\] Show that $f$ has a removable singularity at $z=0$ and compute the value of $f''(i)$.
\end{tcolorbox}
\begin{proof}[\sol]
	content...
\end{proof}

\begin{tcolorbox}[colback=white,colframe=white,arc=5pt,title={\color{black}\bf $\bullet$ Series Expansion of a Complex Function III}]
	
\end{tcolorbox}


\newpage
\begin{tikzpicture}[scale=1.5]
	% draw axis
	\draw[->] (-3,0) -- (3,0) node[right] {$\operatorname{Re}(z)$};
	\draw[->] (0,-3) -- (0,3) node[above] {$\operatorname{Im}(z)$};
	
	% (1) 0 < |z - 1| < 1
	%\draw[dashed, fill=gray!20] (1,0) circle (1);
	%\node at (1.5,0.5) {1};
	
	% (2) 1 < |z| < 2
	%\draw[dashed, fill=gray!40] (0,0) circle (2);
	%\draw[fill=white] (0,0) circle (1);
	%\node at (1.5,-1) {2};
	
	% (3) |z| < 1
	\draw[dashed, fill=gray!60] (0,0) circle (1);
	\node at (-0.7,-0.7) {3};
	
	% (4) |z| > 2
	% Outer region, can be represented with a larger circle
	%\draw[dashed] (0,0) circle (2.5);
	%\node at (-2,2) {4};
\end{tikzpicture}

\footer{Department of Information Security, Cryptography and Mathematics\\
	Collage of Science and Technology\\
	Kookmin University}
\end{document}
